updates

intermediate/Veritas.Intermediate.Store.fsti
@@ -85,7 +85,7 @@ let desc_in_store (st:vstore_raw) (s:inuse_slot_id st) (d:bin_tree_dir) : bool
     | Right -> Some? (VStoreE?.r_in_store (Some?.v (get_slot st s)))
 
 (* if a descendant was added with MAdd, the slot where the descendant was added *)
-let desc_slot (st:vstore_raw) (s:inuse_slot_id st) (d:bin_tree_dir{desc_in_store st s d}): nat
+let desc_slot_raw (st:vstore_raw) (s:inuse_slot_id st) (d:bin_tree_dir{desc_in_store st s d}): nat
   = match d with
     | Left -> Some?.v (VStoreE?.l_in_store (Some?.v (get_slot st s)))
     | Right -> Some?.v (VStoreE?.r_in_store (Some?.v (get_slot st s)))
@@ -95,7 +95,7 @@ let desc_in_store_inv_merkle (st:vstore_raw) (s:merkle_slot_id st) (d:bin_tree_d
   let v = to_merkle_value (stored_value st s) in
   mv_points_to_none v d /\ not (desc_in_store st s d) \/
   mv_points_to_some v d /\ (desc_in_store st s d ==> 
-                            (let ds = desc_slot st s d in
+                            (let ds = desc_slot_raw st s d in
                              ds < Seq.length st /\               // valid slot_id                 
                              (let dk = mv_pointed_key v d in
                               inuse_slot st ds /\                // slot_id in use                              
@@ -124,6 +124,12 @@ let has_key (k:key) (e:option vstore_entry) : bool
   = match e with
     | Some (VStoreE k' _ _ _ _) -> k = k'
     | None -> false
+
+(* desc slot verified version that returns a slot id *)
+let desc_slot (st:vstore) 
+              (s:merkle_slot_id st) 
+              (d:bin_tree_dir{desc_in_store st s d}): slot_id st = 
+  desc_slot_raw st s d
 
 (** vstore update methods **)
 
@@ -166,74 +172,45 @@ val add_to_store_with_desc
 val update_data_value 
   (st:vstore)
   (s:data_slot_id st)
-  (v:value{DVal? v})
-  : Tot (st':vstore {idx_store_update_rel st st' s /\
-                     inuse_slot st' s /\
-                     stored_key st' s = stored_key st s /\                     
-                     stored_value st' s = v})
+  (v:data_value)
+  : Tot (st':vstore {
+        let VStoreE k _ am _ _ = get_inuse_slot st s in
+        (idx_store_update_rel st st' s /\
+         inuse_slot st' s /\
+         get_inuse_slot st' s = VStoreE k (DVal v) am None None)})
 
 (* reset a descendant of a merkle slot *)
 val reset_desc_slot
   (st:vstore)
   (s:merkle_slot_id st)
   (d:bin_tree_dir{desc_in_store st s d})
-  : Tot (st': vstore {Seq.length st = Seq.length st' /\
+  : Tot (st': vstore {idx_store_update_rel st st' s /\
                       inuse_slot st' s /\ 
                       stored_key st' s = stored_key st s /\
                       not (desc_in_store st s d)})
 
+(* two values point to the same key along some dir (or don't point to any) *)
+let points_to_same (v1 v2: merkle_value) (d:bin_tree_dir) = 
+  mv_points_to_none v1 d && mv_points_to_none v2 d ||
+  mv_points_to_some v1 d && mv_points_to_some v2 d && 
+  mv_pointed_key v1 d = mv_pointed_key v2 d
 
-(* update the value of an occupied store slot with a compatible value *)
-let update_value 
+(* update a merkle value with a new value that points to the same keys *)
+val update_merkle_value
   (st:vstore)
-  (s:inuse_slot_id st) 
-  (v:value_type_of (stored_key st s))
-  : Tot (st':vstore {Seq.length st = Seq.length st' /\
-                     inuse_slot st' s /\
-                     stored_value st' s = v})
-  = let Some (VStoreE k _ am l r) = get_slot st s in
-    let st' = update_slot st s (VStoreE k v am l r) in
-    admit()
-    //update_slot st s (VStoreE k v am l r)
-
-let update_value_preserves_length 
-      (st:vstore) 
-      (s:slot_id{store_contains st s}) 
-      (v:value_type_of (stored_key st s)) 
-  : Lemma (let st' = update_value st s v in
-           Seq.length st = Seq.length st')
-          [SMTPat (Seq.length (update_value st s v))]  
-  = ()
-
-let lemma_update_value_preserves_slots
-      (st:vstore) 
-      (s:slot_id{store_contains st s}) 
-      (v:value_type_of (stored_key st s))
-      (s':slot_id)
-  : Lemma (store_contains st s' = store_contains (update_value st s v) s')
-          [SMTPat (store_contains (update_value st s v) s')]
-  = ()
-
-(* update desc in store; we do not have an update that sets desc_in_store to None *)
-let update_desc_in_store
-  (st:vstore)
-  (s:instore_merkle_slot st)
-  (d:bin_tree_dir)
-  (s':slot_id{s' <> s})
-  : Tot (st':vstore {store_contains st' s /\ 
-                     stored_key st' s = stored_key st s /\
-                     desc_in_store st' s d /\
-                     desc_slot st' s d = s'})
-  = let Some (VStoreE k v am ld rd) = get_slot st s in
-    match d with
-    | Left -> update_slot st s (VStoreE k v am (Some s') rd) 
-    | Right -> update_slot st s (VStoreE k v am ld (Some s'))
-
+  (s:merkle_slot_id st)
+  (v:merkle_value {let vold = to_merkle_value (stored_value st s) in
+                   points_to_same v vold Left &&
+                   points_to_same v vold Right})
+  : Tot (st': vstore {idx_store_update_rel st st' s /\
+                      inuse_slot st' s /\
+                      (let VStoreE k _ am ld rd = get_inuse_slot st s in
+                       get_inuse_slot st' s = VStoreE k (MVal v) am ld rd)})
 
 (* remove an entry from a slot; reset slot to unused *)
-let evict_from_store (st:vstore) (s:st_index st)
-  : Tot (st':vstore {not (store_contains st' s)})
-  = Seq.upd st s None
+val evict_from_store (st:vstore) (s:inuse_slot_id st)
+  : Tot (st':vstore {idx_store_update_rel st st' s /\
+                     empty_slot st' s})
 
 (* if the store contains key k, return some entry in the store, otherwise return None *)
 let lookup_key (st:vstore) (k:key) 
@@ -264,174 +241,78 @@ val add_method_of_by_key (st:vstore) (k:key{store_contains_key st k}) : add_meth
 
 (* No duplicate keys in the store *)
 let is_map (st:vstore) =
-  forall (s:slot_id{store_contains st s}) 
-    (s':slot_id{store_contains st s' /\ s' <> s}). 
+  forall (s:inuse_slot_id st) 
+    (s':inuse_slot_id st{s' <> s}). 
         // TODO: this pattern is pretty general -- it may lead to proof performance issues
         {:pattern (Seq.index st s); (Seq.index st s')} 
     stored_key st s <> stored_key st s'
 
 let elim_is_map (st:vstore) 
-                (s:slot_id{store_contains st s})
-                (s':slot_id{store_contains st s' /\ s' <> s})
+                (s:inuse_slot_id st)
+                (s':inuse_slot_id st{s' <> s})
   : Lemma (requires is_map st)
           (ensures stored_key st s ≠ stored_key st s')
   = ()
 
-let points_to_some (st:vstore) (s:instore_merkle_slot st) (d:bin_tree_dir) : bool
-  = let mv = to_merkle_value (stored_value st s) in
-    mv_points_to_some mv d
+(* a store that is a map *)
+let ismap_vstore = st:vstore{is_map st}
 
-let pointed_key (st:vstore) (s:instore_merkle_slot st) (d:bin_tree_dir{points_to_some st s d}) : key
-  = let mv = to_merkle_value (stored_value st s) in
-    mv_pointed_key mv d
+(* updating a data value preserves is_map *)
+val lemma_update_data_value_preserves_is_map
+      (st:ismap_vstore)
+      (s:data_slot_id st)
+      (v:data_value)
+  : Lemma (ensures (is_map (update_data_value st s v)))
+          [SMTPat (update_data_value st s v)]
 
-let store_inv (st:vstore) = 
-  is_map st /\ in_store_inv st
+(* reset desc slot preserves is_map *)
+val lemma_reset_desc_slot_preserves_is_map
+      (st:ismap_vstore)
+      (s:merkle_slot_id st)
+      (d:bin_tree_dir{desc_in_store st s d})
+  : Lemma (ensures (is_map (reset_desc_slot st s d)))
+          [SMTPat (is_map (reset_desc_slot st s d))]
 
-let lemma_update_value_preserves_is_map
-      (st:vstore) 
-      (s:slot_id{store_contains st s}) 
-      (v:value_type_of (stored_key st s)) 
-  : Lemma (requires (is_map st))
-          (ensures (is_map (update_value st s v)))
-          [SMTPat (is_map (update_value st s v))]
-  = ()
-
-let lemma_update_in_store_preserves_is_map
-      (st:vstore) 
-      (s:instore_merkle_slot st) 
-      (d:bin_tree_dir)
-      (s':slot_id)
-  : Lemma (requires (is_map st))
-          (ensures (is_map (update_desc_in_store st s d s')))
-          [SMTPat (is_map (update_desc_in_store st s d s'))]
-  = ()
+val lemma_update_merkle_value
+      (st:ismap_vstore)
+      (s:merkle_slot_id st)
+      (v:merkle_value {let vold = to_merkle_value (stored_value st s) in
+                       points_to_same v vold Left &&
+                       points_to_same v vold Right})
+  : Lemma (ensures (is_map (update_merkle_value st s v)))
+          [SMTPat (is_map (update_merkle_value st s v))]
 
 (* is_map is preserved when adding a new key *)
 val lemma_add_to_store_is_map1
-      (st:vstore) 
-      (s:st_index st{not (store_contains st s)}) 
+      (st:ismap_vstore) 
+      (s:empty_slot_id st) 
       (k:key{not (store_contains_key st k)}) 
       (v:value_type_of k) 
       (am:add_method)
-  : Lemma (requires (is_map st))
-          (ensures (is_map (add_to_store st s k v am)))
+  : Lemma (ensures (is_map (add_to_store st s k v am)))
           [SMTPat (is_map (add_to_store st s k v am))]
 
 (* is_map is violated when adding a duplicate key *)
 val lemma_add_to_store_is_map2
       (st:vstore) 
-      (s:st_index st{not (store_contains st s)}) 
+      (s:empty_slot_id st) 
       (k:key{store_contains_key st k}) 
       (v:value_type_of k) 
       (am:add_method)
   : Lemma (ensures (~ (is_map (add_to_store st s k v am))))
           [SMTPat (is_map (add_to_store st s k v am))]
 
-let lemma_evict_from_store_preserves_is_map (st:vstore) (s:st_index st)
-  : Lemma (requires (is_map st))
-          (ensures (is_map (evict_from_store st s)))
+val lemma_evict_from_store_preserves_is_map (st:ismap_vstore) (s:inuse_slot_id st)
+  : Lemma (ensures (is_map (evict_from_store st s)))
           [SMTPat (is_map (evict_from_store st s))]
-  = ()
-
-(* proving in_store_bit_inv requires a bunch of simple facts about store_contains_key_with_MAdd *)
-
-(* a key is present in a store iff it is present after updating 
-   the store with a new value for some key at some slot *)
-val lemma_update_value_preserves_keys
-      (st:vstore) 
-      (s:slot_id{store_contains st s}) 
-      (v:value_type_of (stored_key st s))
-      (k:key)
-  : Lemma (store_contains_key st k = store_contains_key (update_value st s v) k)
-          [SMTPat (store_contains_key (update_value st s v) k)]
-
-val lemma_update_value_preserves_key_with_MAdd
-  (st:vstore)
-  (s:slot_id{store_contains st s}) 
-  (v:value_type_of (stored_key st s))
-  (k:key)
-  : Lemma (ensures store_contains_key_with_MAdd st k = 
-                     store_contains_key_with_MAdd (update_value st s v) k)
-          [SMTPat (store_contains_key_with_MAdd (update_value st s v) k)]
-
-val lemma_add_different_key_to_store_preserves_keys_with_MAdd
-  (st:vstore)
-  (s:st_index st{not (store_contains st s)}) 
-  (k:key)
-  (v:value_type_of k)
-  (k0:key)
-  : Lemma (requires k <> k0)
-          (ensures store_contains_key_with_MAdd st k0 =
-                     store_contains_key_with_MAdd (add_to_store st s k v Spec.MAdd) k0)
-          [SMTPat (store_contains_key_with_MAdd (add_to_store st s k v Spec.MAdd) k0)]
-
-val lemma_add_to_store_BAdd_preserves_key_with_MAdd
-  (st:vstore)
-  (s:st_index st{not (store_contains st s)}) 
-  (k:key{not (store_contains_key st k)})
-  (v:value_type_of k)
-  (k0:key)
-  : Lemma (ensures store_contains_key_with_MAdd st k0 = 
-                     store_contains_key_with_MAdd (add_to_store st s k v Spec.BAdd) k0)
-          [SMTPat (store_contains_key_with_MAdd (add_to_store st s k v Spec.BAdd) k0)]
-
-val lemma_add_to_store_MAdd_adds_key_with_MAdd
-  (st:vstore)
-  (s:st_index st{not (store_contains st s)}) 
-  (k:key{not (store_contains_key st k)})
-  (v:value_type_of k)
-  : Lemma (ensures store_contains_key_with_MAdd (add_to_store st s k v Spec.MAdd) k)
-          [SMTPat (store_contains_key_with_MAdd (add_to_store st s k v Spec.MAdd) k)]
-
-val lemma_update_in_store_preserves_keys
-  (st:vstore)
-  (s:st_index st{store_contains st s}) 
-  (d:bin_tree_dir)
-  (b:bool)
-  (k:key)
-  : Lemma (ensures store_contains_key st k = store_contains_key (update_in_store st s d b) k)
-          [SMTPat (store_contains_key (update_in_store st s d b) k)]
-
-val lemma_update_in_store_preserves_key_with_MAdd
-  (st:vstore)
-  (s:st_index st{store_contains st s}) 
-  (d:bin_tree_dir)
-  (b:bool)
-  (k:key)
-  : Lemma (ensures store_contains_key_with_MAdd st k = 
-                     store_contains_key_with_MAdd (update_in_store st s d b) k)
-          [SMTPat (store_contains_key_with_MAdd (update_in_store st s d b) k)]
-
-val lemma_evict_from_store_evicts_key
-  (st:vstore)
-  (s:st_index st{store_contains st s}) 
-  : Lemma (requires is_map st)
-          (ensures not (store_contains_key (evict_from_store st s) (stored_key st s)))
-          [SMTPat (store_contains_key (evict_from_store st s) (stored_key st s))]
-
-val lemma_evict_from_store_preserves_key_with_MAdd
-  (st:vstore)
-  (s:st_index st{store_contains st s}) 
-  (k:key)
-  : Lemma (requires (k <> stored_key st s))
-          (ensures (store_contains_key_with_MAdd st k = store_contains_key_with_MAdd (evict_from_store st s) k))
-          [SMTPat (store_contains_key_with_MAdd (evict_from_store st s) k)]
-
-val lemma_evict_from_store_BAdd_preserves_key_with_MAdd
-  (st:vstore{is_map st})
-  (s:st_index st{store_contains st s}) 
-  (k:key)
-  : Lemma (requires (add_method_of st s = Spec.BAdd))
-          (ensures (store_contains_key_with_MAdd st k = store_contains_key_with_MAdd (evict_from_store st s) k))
-          [SMTPat (store_contains_key_with_MAdd (evict_from_store st s) k)]
 
 (*** Relation w/ Spec-level Stores ***)
 
 (* slot_id s is equivalent to key k *)
-let slot_key_equiv (st:vstore) (s:slot_id) (k:key) : bool =
-  store_contains st s && stored_key st s = k 
+let slot_key_equiv (st:vstore) (s:slot_id st) (k:key) : bool =
+  inuse_slot st s && stored_key st s = k 
 
+(*
 (* if s contains k, it continues to contain k after an unrelated update *)
 val lemma_slot_key_equiv_update_value 
       (st:vstore) 
@@ -442,16 +323,17 @@ val lemma_slot_key_equiv_update_value
   : Lemma (requires (slot_key_equiv st s k /\ s <> s'))
           (ensures (slot_key_equiv (update_value st s' v) s k))
           [SMTPat (slot_key_equiv (update_value st s' v) s k)]
+*)
 
 (* convert a slot-indexed store to a key-indexed store *)
-val as_map (st:vstore{is_map st}) : Spec.vstore
+val as_map (st:ismap_vstore) : Spec.vstore
 
 val lemma_as_map_empty (n:nat) 
   : Lemma (ensures (let st = empty_store n in
                      forall (k:key). as_map st k = None))
           (decreases n)
 
-val lemma_as_map_slot_key_equiv (st:vstore{is_map st}) (s:slot_id) (k:key)
+val lemma_as_map_slot_key_equiv (st:ismap_vstore) (s:slot_id st) (k:key)
   : Lemma (requires (slot_key_equiv st s k)) 
           (ensures (Spec.store_contains (as_map st) k /\
                     stored_value st s = Spec.stored_value (as_map st) k /\
@@ -477,6 +359,7 @@ val lemma_store_rel_add_method_of (st:vstore) (st':Spec.vstore) (k:key)
           (ensures (add_method_of_by_key st k = Spec.add_method_of st' k))
           [SMTPat (add_method_of_by_key st k); SMTPat (Spec.add_method_of st' k)]
 
+(*
 val lemma_store_rel_update_value (st:vstore) (st':Spec.vstore) (s:slot_id) (k:key) (v:value_type_of k)
   : Lemma (requires (store_rel st st' /\ slot_key_equiv st s k))
           (ensures (store_rel (update_value st s v) (Spec.update_store st' k v)))
@@ -486,16 +369,20 @@ val lemma_store_rel_update_in_store (st:vstore) (st':Spec.vstore) (s:slot_id) (d
   : Lemma (requires (store_rel st st' /\ store_contains st s))
           (ensures (store_rel (update_in_store st s d b) st'))
           [SMTPat (store_rel (update_in_store st s d b) st')]
+*)
 
-val lemma_store_rel_add_to_store (st:vstore) (st':Spec.vstore) (s:st_index st) (k:key) (v:value_type_of k) (am:add_method)
-  : Lemma (requires (store_rel st st' /\ not (store_contains st s) /\ not (Spec.store_contains st' k)))
+val lemma_store_rel_add_to_store 
+      (st:vstore) 
+      (st':Spec.vstore) 
+      (s:empty_slot_id st) 
+      (k:key) 
+      (v:value_type_of k) 
+      (am:add_method)
+  : Lemma (requires (store_rel st st' /\ not (Spec.store_contains st' k)))
           (ensures (store_rel (add_to_store st s k v am) (Spec.add_to_store st' k v am)))
           [SMTPat (add_to_store st s k v am); SMTPat (Spec.add_to_store st' k v am)]
 
-val lemma_store_rel_evict_from_store (st:vstore) (st':Spec.vstore) (s:st_index st) (k:key)
+val lemma_store_rel_evict_from_store (st:vstore) (st':Spec.vstore) (s:slot_id st) (k:key)
   : Lemma (requires (store_rel st st' /\ slot_key_equiv st s k))
           (ensures (store_rel (evict_from_store st s) (Spec.evict_from_store st' k)))
           [SMTPat (evict_from_store st s); SMTPat (Spec.evict_from_store st' k)]
-
-
-
